(Almost) Finish forward simulation proof between ORD-RES-2 and ORD-RES-3 up to determinacy of resolvant

Simulation_SCLFOL_Ordered_Resolution/Simulation.thy
@@ -4704,6 +4704,297 @@ definition ord_res_2_measure where
 lemma tranclp_if_relpowp: "n \<noteq> 0 \<Longrightarrow> (R ^^ n) x y \<Longrightarrow> R\<^sup>+\<^sup>+ x y"
   by (meson bot_nat_0.not_eq_extremum tranclp_power)
 
+lemma clause_true_if_resolved_true:
+  assumes
+    "(ground_resolution D)\<^sup>+\<^sup>+ C DC" and
+    D_productive: "ord_res.production N D \<noteq> {}" and
+    C_true: "ord_res_Interp N DC \<TTurnstile> DC"
+  shows "ord_res_Interp N C \<TTurnstile> C"
+proof -
+  obtain n where
+    steps: "(ground_resolution D ^^ Suc n) C DC"
+    using \<open>(ground_resolution D)\<^sup>+\<^sup>+ C DC\<close>
+    by (metis less_not_refl not0_implies_Suc tranclp_power)
+
+  obtain m A D' C' where
+    "n \<le> m" and
+    "ord_res.is_strictly_maximal_lit (Pos A) D" and
+    "ord_res.is_maximal_lit (Neg A) C" and
+    "D = add_mset (Pos A) D'" and
+    "C = replicate_mset (Suc m) (Neg A) + C'" and
+    "Neg A \<notin># C'" and
+    "DC = repeat_mset (Suc n) D' + replicate_mset (m - n) (Neg A) + C'"
+    using relpowp_ground_resolutionD[OF Suc_not_Zero steps]
+    by (metis diff_Suc_Suc Suc_le_mono)
+
+  have "Neg A \<notin># D'"
+    by (metis \<open>D = add_mset (Pos A) D'\<close> \<open>ord_res.is_strictly_maximal_lit (Pos A) D\<close>
+        ord_res.less_lit_simps(4) linorder_lit.is_greatest_in_mset_iff linorder_trm.eq_refl
+        linorder_trm.leD remove1_mset_add_mset_If)
+  
+  have "DC \<prec>\<^sub>c C"
+  proof (cases "m = n")
+    case True
+    show ?thesis
+    proof (intro one_step_implies_multp[of _ _ _ "{#}", simplified] ballI)
+      show "C \<noteq> {#}"
+        by (simp add: \<open>C = replicate_mset (Suc m) (Neg A) + C'\<close>)
+    next
+      fix L
+      assume "L \<in># DC"
+      hence "L \<in># D' \<or> L \<in># C'"
+        unfolding \<open>DC = repeat_mset (Suc n) D' + replicate_mset (m - n) (Neg A) + C'\<close> \<open>m = n\<close>
+        using member_mset_repeat_msetD by fastforce
+      hence "L \<prec>\<^sub>l Neg A"
+        using \<open>ord_res.is_strictly_maximal_lit (Pos A) D\<close> \<open>ord_res.is_maximal_lit (Neg A) C\<close>
+        unfolding \<open>D = add_mset (Pos A) D'\<close> \<open>C = replicate_mset (Suc m) (Neg A) + C'\<close>
+        unfolding linorder_lit.is_maximal_in_mset_iff linorder_lit.is_greatest_in_mset_iff
+        by (metis \<open>Neg A \<notin># C'\<close> add_mset_remove_trivial ord_res.less_lit_simps(4)
+            linorder_lit.antisym_conv3 linorder_lit.dual_order.strict_trans
+            linorder_trm.dual_order.asym union_iff)
+
+      moreover have "Neg A \<in># C"
+        by (simp add: \<open>C = replicate_mset (Suc m) (Neg A) + C'\<close>)
+
+      ultimately show "\<exists>K \<in># C. L \<prec>\<^sub>l K"
+        by metis
+    qed
+  next
+    case False
+    hence "n < m"
+      using \<open>n \<le> m\<close> by presburger
+
+    have "multp\<^sub>H\<^sub>O (\<prec>\<^sub>l) DC C"
+    proof (rule linorder_lit.multp\<^sub>H\<^sub>O_if_same_maximal_and_count_lt)
+      show "ord_res.is_maximal_lit (Neg A) DC"
+        unfolding linorder_lit.is_maximal_in_mset_iff
+      proof (intro conjI ballI impI)
+        show "Neg A \<in># DC"
+          unfolding \<open>DC = repeat_mset (Suc n) D' + replicate_mset (m - n) (Neg A) + C'\<close>
+          using \<open>n < m\<close> by simp
+      next
+        fix L
+        assume "L \<in># DC" and "L \<noteq> Neg A"
+        hence "L \<in># D' \<or> L \<in># C'"
+          unfolding \<open>DC = repeat_mset (Suc n) D' + replicate_mset (m - n) (Neg A) + C'\<close>
+          by (metis in_replicate_mset member_mset_repeat_msetD union_iff)
+        thus "\<not> Neg A \<prec>\<^sub>l L"
+          using \<open>ord_res.is_strictly_maximal_lit (Pos A) D\<close> \<open>ord_res.is_maximal_lit (Neg A) C\<close>
+          unfolding \<open>D = add_mset (Pos A) D'\<close> \<open>C = replicate_mset (Suc m) (Neg A) + C'\<close>
+          unfolding linorder_lit.is_maximal_in_mset_iff linorder_lit.is_greatest_in_mset_iff
+          by (metis \<open>L \<noteq> Neg A\<close> add_mset_diff_bothsides diff_zero
+              linorder_lit.dual_order.strict_trans linorder_trm.less_irrefl
+              ord_res.less_lit_simps(4) union_iff)
+      qed
+    next
+      show "ord_res.is_maximal_lit (Neg A) C"
+        using \<open>ord_res.is_maximal_lit (Neg A) C\<close> .
+    next
+      have "count DC (Neg A) = count (repeat_mset (Suc n) D') (Neg A) +
+      count (replicate_mset (m - n) (Neg A)) (Neg A) + count C' (Neg A)"
+        unfolding \<open>DC = repeat_mset (Suc n) D' + replicate_mset (m - n) (Neg A) + C'\<close> by simp
+      also have "\<dots> = count D' (Neg A) * Suc n + count {#Neg A#} (Neg A) * (m - n) + count C' (Neg A)"
+        by simp
+      also have "\<dots> = 0 * Suc n + 1 * (m - n) + 0"
+        by (simp add: \<open>Neg A \<notin># C'\<close> \<open>Neg A \<notin># D'\<close> count_eq_zero_iff)
+      also have "\<dots> = m - n"
+        by presburger
+      also have "\<dots> < Suc m"
+        by presburger
+      also have "\<dots> = 1 * Suc m + 0"
+        by presburger
+      also have "\<dots> = count {#Neg A#} (Neg A) * Suc m + count C' (Neg A)"
+        by (simp add: \<open>Neg A \<notin># C'\<close> count_eq_zero_iff)
+      also have "\<dots> = count (replicate_mset (Suc m) (Neg A)) (Neg A) + count C' (Neg A)"
+        by simp
+      also have "\<dots> = count C (Neg A)"
+        unfolding \<open>C = replicate_mset (Suc m) (Neg A) + C'\<close> by simp
+      finally show "count DC (Neg A) < count C (Neg A)" .
+    qed
+    thus ?thesis
+      by (simp add: multp\<^sub>D\<^sub>M_imp_multp multp\<^sub>H\<^sub>O_imp_multp\<^sub>D\<^sub>M)
+  qed
+
+  with C_true have "ord_res_Interp N C \<TTurnstile> DC"
+    using ord_res.entailed_clause_stays_entailed by metis
+
+  thus "ord_res_Interp N C \<TTurnstile> C"
+    unfolding true_cls_def
+  proof (elim bexE)
+    fix L
+    assume
+      L_in: "L \<in># DC" and
+      L_true: "ord_res_Interp N C \<TTurnstile>l L"
+
+    from L_in have "L \<in># D' \<or> L = Neg A \<or> L \<in># C'"
+      unfolding \<open>DC = repeat_mset (Suc n) D' + replicate_mset (m - n) (Neg A) + C'\<close>
+      by (metis in_replicate_mset member_mset_repeat_msetD union_iff)
+
+    moreover have "L \<notin># D'"
+    proof (rule notI)
+      assume "L \<in># D'"
+
+      moreover have "\<not> ord_res.interp N (add_mset (Pos A) D') \<TTurnstile> add_mset (Pos A) D'"
+        using D_productive[unfolded \<open>D = add_mset (Pos A) D'\<close>]
+        unfolding ord_res.production_unfold
+        by fast
+
+      ultimately have "\<not> ord_res.interp N (add_mset (Pos A) D') \<TTurnstile>l L"
+        by auto
+
+      have "L \<prec>\<^sub>l Pos A"
+        using \<open>D = add_mset (Pos A) D'\<close> \<open>L \<in># D'\<close> \<open>ord_res.is_strictly_maximal_lit (Pos A) D\<close>
+          linorder_lit.is_greatest_in_mset_iff by fastforce
+
+      have "\<not> ord_res_Interp N C \<TTurnstile>l L"
+      proof (cases L)
+        case (Pos B)
+        hence "B \<notin> ord_res.interp N (add_mset (Pos A) D')"
+          using \<open>\<not> ord_res.interp N (add_mset (Pos A) D') \<TTurnstile>l L\<close> by simp
+
+        moreover have "add_mset (Pos A) D' \<prec>\<^sub>c C"
+          by (metis \<open>D = add_mset (Pos A) D'\<close> \<open>\<And>thesis. (\<And>m A D' C'. \<lbrakk>n \<le> m; ord_res.is_strictly_maximal_lit (Pos A) D; ord_res.is_maximal_lit (Neg A) C; D = add_mset (Pos A) D'; C = replicate_mset (Suc m) (Neg A) + C'; Neg A \<notin># C'; DC = repeat_mset (Suc n) D' + replicate_mset (m - n) (Neg A) + C'\<rbrakk> \<Longrightarrow> thesis) \<Longrightarrow> thesis\<close> linorder_lit.is_maximal_in_mset_if_is_greatest_in_mset linorder_lit.multp\<^sub>H\<^sub>O_if_maximal_less_that_maximal multp\<^sub>D\<^sub>M_imp_multp multp\<^sub>H\<^sub>O_imp_multp\<^sub>D\<^sub>M ord_res.less_lit_simps(2) reflclp_iff)
+
+        ultimately have "B \<notin> ord_res.interp N C"
+          using \<open>L \<prec>\<^sub>l Pos A\<close>[unfolded Pos, simplified]
+          using ord_res.interp_fixed_for_smaller_literals
+          by (metis \<open>D = add_mset (Pos A) D'\<close> \<open>ord_res.is_strictly_maximal_lit (Pos A) D\<close>
+              linorder_lit.is_maximal_in_mset_if_is_greatest_in_mset literal.sel(1))
+
+        moreover have "B \<notin> ord_res.production N C"
+          by (metis Uniq_D \<open>ord_res.is_maximal_lit (Neg A) C\<close> ground_ordered_resolution_calculus.mem_productionE linorder_lit.Uniq_is_maximal_in_mset linorder_lit.is_maximal_in_mset_if_is_greatest_in_mset literal.simps(4) ord_res.ground_ordered_resolution_calculus_axioms)
+
+        ultimately show ?thesis
+          unfolding Pos by simp
+      next
+        case (Neg B)
+        hence "B \<in> ord_res.interp N (add_mset (Pos A) D')"
+          using \<open>\<not> ord_res.interp N (add_mset (Pos A) D') \<TTurnstile>l L\<close> by simp
+
+        moreover have "add_mset (Pos A) D' \<prec>\<^sub>c C"
+          by (metis \<open>D = add_mset (Pos A) D'\<close> \<open>\<And>thesis. (\<And>m A D' C'. \<lbrakk>n \<le> m; ord_res.is_strictly_maximal_lit (Pos A) D; ord_res.is_maximal_lit (Neg A) C; D = add_mset (Pos A) D'; C = replicate_mset (Suc m) (Neg A) + C'; Neg A \<notin># C'; DC = repeat_mset (Suc n) D' + replicate_mset (m - n) (Neg A) + C'\<rbrakk> \<Longrightarrow> thesis) \<Longrightarrow> thesis\<close> linorder_lit.is_maximal_in_mset_if_is_greatest_in_mset linorder_lit.multp\<^sub>H\<^sub>O_if_maximal_less_that_maximal multp\<^sub>D\<^sub>M_imp_multp multp\<^sub>H\<^sub>O_imp_multp\<^sub>D\<^sub>M ord_res.less_lit_simps(2) reflclp_iff)
+
+        ultimately have "B \<in> ord_res.interp N C"
+          by (metis Un_iff ord_res.not_interp_to_Interp_imp_le linorder_cls.leD)
+
+        then show ?thesis
+          unfolding Neg
+          by simp
+      qed
+
+      with L_true show False
+        by contradiction
+    qed
+
+    ultimately have "L \<in># C"
+      unfolding \<open>C = replicate_mset (Suc m) (Neg A) + C'\<close> by simp
+
+    with L_true show "\<exists>L \<in># C. ord_res_Interp N C \<TTurnstile>l L"
+      by metis
+  qed
+qed
+
+lemma clause_true_if_eres_true:
+  assumes
+    "(ground_resolution D1)\<^sup>+\<^sup>+ D2 C" and
+    "C \<noteq> eres D1 C" and
+    eres_C_true: "ord_res_Interp N (eres D1 C) \<TTurnstile> eres D1 C"
+  shows "ord_res_Interp N C \<TTurnstile> C"
+proof -
+  obtain n where
+    steps: "(ground_resolution D1 ^^ Suc n) D2 C"
+    using \<open>(ground_resolution D1)\<^sup>+\<^sup>+ D2 C\<close>
+    by (metis less_not_refl not0_implies_Suc tranclp_power)
+
+  obtain m A D' C' where
+    "n \<le> m" and
+    "ord_res.is_strictly_maximal_lit (Pos A) D1" and
+    "ord_res.is_maximal_lit (Neg A) D2" and
+    "D1 = add_mset (Pos A) D'" and
+    "D2 = replicate_mset (Suc m) (Neg A) + C'" and
+    "Neg A \<notin># C'" and
+    "C = repeat_mset (Suc n) D' + replicate_mset (m - n) (Neg A) + C'"
+    using relpowp_ground_resolutionD[OF Suc_not_Zero steps]
+    by (metis diff_Suc_Suc Suc_le_mono)
+
+  have "Neg A \<notin># D'"
+    by (metis \<open>D1 = add_mset (Pos A) D'\<close> \<open>ord_res.is_strictly_maximal_lit (Pos A) D1\<close>
+        ord_res.less_lit_simps(4) linorder_lit.is_greatest_in_mset_iff linorder_trm.eq_refl
+        linorder_trm.leD remove1_mset_add_mset_If)
+
+  obtain m' C'' where
+    "C = replicate_mset (Suc m') (Neg A) + C''" and
+    "Neg A \<notin># C''" and
+    "eres D1 C = repeat_mset (Suc m') D' + C''"
+    using \<open>C \<noteq> eres D1 C\<close> eres_not_identD
+    using \<open>ord_res.is_strictly_maximal_lit (Pos A) D1\<close> linorder_lit.Uniq_is_greatest_in_mset
+    using \<open>D1 = add_mset (Pos A) D'\<close>
+    by (metis Uniq_D add_mset_remove_trivial literal.inject(1))
+
+  have "m - n = Suc m'"
+  proof -
+    have "count C (Neg A) = count (repeat_mset (Suc n) D') (Neg A) +
+              count (replicate_mset (m - n) (Neg A)) (Neg A) + count C' (Neg A)"
+      using \<open>C = repeat_mset (Suc n) D' + replicate_mset (m - n) (Neg A) + C'\<close> by simp
+    also have "\<dots> = count D' (Neg A) * Suc n + count {#Neg A#} (Neg A) * (m - n) +
+              count C' (Neg A)"
+      by simp
+    also have "\<dots> = 0 * Suc n + 1 * (m - n) + 0"
+      using \<open>Neg A \<notin># D'\<close> \<open>Neg A \<notin># C'\<close> by (simp add: count_eq_zero_iff)
+    also have "\<dots> = m - n"
+      by presburger
+    finally have "count C (Neg A) = m - n" .
+
+    have "count C (Neg A) = count (replicate_mset (Suc m') (Neg A)) (Neg A) +
+              count C'' (Neg A)"
+      using \<open>C = replicate_mset (Suc m') (Neg A) + C''\<close> by simp
+    also have "\<dots> = count {#Neg A#} (Neg A) * Suc m' + count C'' (Neg A)"
+      by simp
+    also have "\<dots> = 1 * Suc m' + 0"
+      using \<open>Neg A \<notin># C''\<close> by (simp add: count_eq_zero_iff)
+    also have "\<dots> = Suc m'"
+      by presburger
+    finally have "count C (Neg A) = Suc m'" .
+
+    show ?thesis
+      using \<open>count C (Neg A) = m - n\<close> \<open>count C (Neg A) = Suc m'\<close> by argo
+  qed
+
+  hence "C'' = repeat_mset (Suc n) D' + C'"
+    using \<open>C = repeat_mset (Suc n) D' + replicate_mset (m - n) (Neg A) + C'\<close>
+      \<open>C = replicate_mset (Suc m') (Neg A) + C''\<close>
+    by simp
+
+  hence eres_D1_C_eq: "eres D1 C = repeat_mset (Suc m' + Suc n) D' + C'"
+    using \<open>eres D1 C = repeat_mset (Suc m') D' + C''\<close> by simp
+
+  have "ord_res_Interp N (eres D1 C) \<TTurnstile> eres D1 C"
+    using eres_C_true .
+
+  moreover have "eres D1 C \<prec>\<^sub>c C"
+    using eres_le[of D1 C] \<open>C \<noteq> eres D1 C\<close> by order
+
+  ultimately have "ord_res_Interp N C \<TTurnstile> eres D1 C"
+    using ord_res.entailed_clause_stays_entailed by metis
+
+  thus "ord_res_Interp N C \<TTurnstile> C"
+    unfolding true_cls_def
+  proof (elim bexE)
+    fix L
+    assume
+      L_in: "L \<in># eres D1 C" and
+      L_true: "ord_res_Interp N C \<TTurnstile>l L"
+
+    from L_in have "L \<in># D' \<or> L \<in># C'"
+      unfolding eres_D1_C_eq
+      using member_mset_repeat_msetD by fastforce
+    hence "L \<in># C"
+      by (auto simp: \<open>C = repeat_mset (Suc n) D' + replicate_mset (m - n) (Neg A) + C'\<close>)
+    with L_true show "\<exists>L \<in># C. ord_res_Interp N C \<TTurnstile>l L"
+      by metis
+  qed
+qed
+
 interpretation bisimulation_with_measuring_function' where
   step1 = ord_res_2 and final1 = ord_res_2_final and
   step2 = ord_res_3 and final2 = ord_res_3_final and
@@ -4991,99 +5282,8 @@ next
         have False
         proof (cases "ord_res_Interp (fset (N |\<union>| U\<^sub>e\<^sub>r |\<union>| U\<^sub>e\<^sub>f)) (eres D1 C) \<TTurnstile> eres D1 C")
           case eres_C_true: True
-
-          obtain n where
-            steps: "(ground_resolution D1 ^^ Suc n) D2 C"
-            using \<open>(ground_resolution D1)\<^sup>+\<^sup>+ D2 C\<close>
-            by (metis less_not_refl not0_implies_Suc tranclp_power)
-
-          obtain m A D' C' where
-            "n \<le> m" and
-            "ord_res.is_strictly_maximal_lit (Pos A) D1" and
-            "ord_res.is_maximal_lit (Neg A) D2" and
-            "D1 = add_mset (Pos A) D'" and
-            "D2 = replicate_mset (Suc m) (Neg A) + C'" and
-            "Neg A \<notin># C'" and
-            "C = repeat_mset (Suc n) D' + replicate_mset (m - n) (Neg A) + C'"
-            using relpowp_ground_resolutionD[OF Suc_not_Zero steps]
-            by (metis diff_Suc_Suc Suc_le_mono)
-
-          have "Neg A \<notin># D'"
-            by (metis \<open>D1 = add_mset (Pos A) D'\<close> \<open>ord_res.is_strictly_maximal_lit (Pos A) D1\<close>
-                ord_res.less_lit_simps(4) linorder_lit.is_greatest_in_mset_iff linorder_trm.eq_refl
-                linorder_trm.leD remove1_mset_add_mset_If)
-
-          obtain m' C'' where
-            "C = replicate_mset (Suc m') (Neg A) + C''" and
-            "Neg A \<notin># C''" and
-            "eres D1 C = repeat_mset (Suc m') D' + C''"
-            using \<open>C \<noteq> eres D1 C\<close> eres_not_identD
-            using \<open>ord_res.is_strictly_maximal_lit (Pos A) D1\<close> linorder_lit.Uniq_is_greatest_in_mset
-            using \<open>D1 = add_mset (Pos A) D'\<close>
-            by (metis Uniq_D add_mset_remove_trivial literal.inject(1))
-
-          have "m - n = Suc m'"
-          proof -
-            have "count C (Neg A) = count (repeat_mset (Suc n) D') (Neg A) +
-              count (replicate_mset (m - n) (Neg A)) (Neg A) + count C' (Neg A)"
-              using \<open>C = repeat_mset (Suc n) D' + replicate_mset (m - n) (Neg A) + C'\<close> by simp
-            also have "\<dots> = count D' (Neg A) * Suc n + count {#Neg A#} (Neg A) * (m - n) +
-              count C' (Neg A)"
-              by simp
-            also have "\<dots> = 0 * Suc n + 1 * (m - n) + 0"
-              using \<open>Neg A \<notin># D'\<close> \<open>Neg A \<notin># C'\<close> by (simp add: count_eq_zero_iff)
-            also have "\<dots> = m - n"
-              by presburger
-            finally have "count C (Neg A) = m - n" .
-
-            have "count C (Neg A) = count (replicate_mset (Suc m') (Neg A)) (Neg A) +
-              count C'' (Neg A)"
-              using \<open>C = replicate_mset (Suc m') (Neg A) + C''\<close> by simp
-            also have "\<dots> = count {#Neg A#} (Neg A) * Suc m' + count C'' (Neg A)"
-              by simp
-            also have "\<dots> = 1 * Suc m' + 0"
-              using \<open>Neg A \<notin># C''\<close> by (simp add: count_eq_zero_iff)
-            also have "\<dots> = Suc m'"
-              by presburger
-            finally have "count C (Neg A) = Suc m'" .
-
-            show ?thesis
-              using \<open>count C (Neg A) = m - n\<close> \<open>count C (Neg A) = Suc m'\<close> by argo
-          qed
-
-          hence "C'' = repeat_mset (Suc n) D' + C'"
-            using \<open>C = repeat_mset (Suc n) D' + replicate_mset (m - n) (Neg A) + C'\<close>
-              \<open>C = replicate_mset (Suc m') (Neg A) + C''\<close>
-            by simp
-
-          hence eres_D1_C_eq: "eres D1 C = repeat_mset (Suc m' + Suc n) D' + C'"
-            using \<open>eres D1 C = repeat_mset (Suc m') D' + C''\<close> by simp
-
-          have "ord_res_Interp (fset (N |\<union>| U\<^sub>e\<^sub>r |\<union>| U\<^sub>e\<^sub>f)) (eres D1 C) \<TTurnstile> eres D1 C"
-            using eres_C_true unfolding Interp_N_U\<^sub>r_U\<^sub>e\<^sub>f_eq_Interp_N_U\<^sub>e\<^sub>r_U\<^sub>e\<^sub>f .
-
-          moreover have "eres D1 C \<prec>\<^sub>c C"
-            using eres_le[of D1 C] \<open>C \<noteq> eres D1 C\<close> by order
-
-          ultimately have "ord_res_Interp (fset (N |\<union>| U\<^sub>e\<^sub>r |\<union>| U\<^sub>e\<^sub>f)) C \<TTurnstile> eres D1 C"
-            using ord_res.entailed_clause_stays_entailed by metis
-
           hence "ord_res_Interp (fset (N |\<union>| U\<^sub>e\<^sub>r |\<union>| U\<^sub>e\<^sub>f)) C \<TTurnstile> C"
-            unfolding true_cls_def
-          proof (elim bexE)
-            fix L
-            assume
-              L_in: "L \<in># eres D1 C" and
-              L_true: "ord_res_Interp (fset (N |\<union>| U\<^sub>e\<^sub>r |\<union>| U\<^sub>e\<^sub>f)) C \<TTurnstile>l L"
-
-            from L_in have "L \<in># D' \<or> L \<in># C'"
-              unfolding eres_D1_C_eq
-              using member_mset_repeat_msetD by fastforce
-            hence "L \<in># C"
-              by (auto simp: \<open>C = repeat_mset (Suc n) D' + replicate_mset (m - n) (Neg A) + C'\<close>)
-            with L_true show "\<exists>L \<in># C. ord_res_Interp (fset (N |\<union>| U\<^sub>e\<^sub>r |\<union>| U\<^sub>e\<^sub>f)) C \<TTurnstile>l L"
-              by metis
-          qed
+            using \<open>(ground_resolution D1)\<^sup>+\<^sup>+ D2 C\<close> clause_true_if_eres_true by metis
 
           moreover have "\<not> ord_res_Interp (fset (N |\<union>| U\<^sub>e\<^sub>r |\<union>| U\<^sub>e\<^sub>f)) C \<TTurnstile> C"
             using C_least_false
@@ -5399,6 +5599,25 @@ next
               unfolding is_least_false_clause_def linorder_cls.is_least_in_ffilter_iff
               by argo
 
+            hence "\<not> ord_res_Interp (fset (N |\<union>| U\<^sub>r |\<union>| U\<^sub>e\<^sub>f)) DC \<TTurnstile> DC"
+            proof (rule contrapos_nn)
+              assume "ord_res_Interp (fset (N |\<union>| U\<^sub>r |\<union>| U\<^sub>e\<^sub>f)) DC \<TTurnstile> DC"
+
+              moreover have "DC \<prec>\<^sub>c C"
+                using \<open>ord_res.ground_resolution C D DC\<close>
+                  ord_res.ground_resolution_smaller_conclusion
+                by metis
+
+              ultimately have "ord_res_Interp (fset (N |\<union>| U\<^sub>r |\<union>| U\<^sub>e\<^sub>f)) C \<TTurnstile> DC"
+                using ord_res.entailed_clause_stays_entailed by metis
+
+              then show "ord_res_Interp (fset (N |\<union>| U\<^sub>r |\<union>| U\<^sub>e\<^sub>f)) C \<TTurnstile> C"
+                using clause_true_if_resolved_true
+                using \<open>ground_resolution D C DC\<close> \<open>ord_res_Interp (fset (N |\<union>| U\<^sub>r |\<union>| U\<^sub>e\<^sub>f)) DC \<TTurnstile> DC\<close>
+                  \<open>ord_res.production (fset (N |\<union>| U\<^sub>r |\<union>| U\<^sub>e\<^sub>f)) D = {atm_of L}\<close>
+                by fastforce
+            qed
+
             moreover have "ord_res_Interp (fset (N |\<union>| U\<^sub>r' |\<union>| U\<^sub>e\<^sub>f)) x =
               ord_res_Interp (fset (N |\<union>| U\<^sub>r |\<union>| U\<^sub>e\<^sub>f)) x" for x
             proof -
@@ -5413,18 +5632,8 @@ next
                 by simp
             qed
 
-            ultimately have "\<not> ord_res_Interp (fset (N |\<union>| U\<^sub>r' |\<union>| U\<^sub>e\<^sub>f)) C \<TTurnstile> C"
+            ultimately show "\<not> ord_res_Interp (fset (N |\<union>| U\<^sub>r' |\<union>| U\<^sub>e\<^sub>f)) DC \<TTurnstile> DC"
               by metis
-
-            thus "\<not> ord_res_Interp (fset (N |\<union>| U\<^sub>r' |\<union>| U\<^sub>e\<^sub>f)) DC \<TTurnstile> DC"
-            proof (rule contrapos_nn)
-              assume "ord_res_Interp (fset (N |\<union>| U\<^sub>r' |\<union>| U\<^sub>e\<^sub>f)) DC \<TTurnstile> DC"
-              then show "ord_res_Interp (fset (N |\<union>| U\<^sub>r' |\<union>| U\<^sub>e\<^sub>f)) C \<TTurnstile> C"
-                \<comment> \<open>DC is not exhaustively factorized, hence it is not productive. We know by
-                definition of resolution that DC consists only of false literals from D or literals
-                from C, which are all false because we know C to be the least false clause.\<close>
-                sorry
-            qed
           next
             fix y
             assume
